Introduce the monad transformer typeclass

theories/Control.v
@@ -95,6 +95,16 @@ Class Monad
      ; monad_is_bind :> Bind m
      }.
 
+(** * Monad Transformer
+
+ *)
+
+Class MonadTrans
+      (t: forall (m: Type -> Type) `{Monad m}, Type -> Type)
+  := { monad_trans_is_monad (m: Type -> Type) `{Monad m} :> Monad (t m)
+     ; lift (m: Type -> Type) `{Monad m} (a: Type): m a -> t m a
+     }.
+
 Notation "a <- p ; q" :=
   (bind p (fun a => q)) (at level 99, right associativity, p at next level)
   : free_control_scope.
