theories/Control/Identity.v
@@ -1,0 +1,57 @@
+Require Import FreeSpec.Control.
+
+Definition Identity
+           (a: Type)
+  := a.
+
+Definition identity_map
+           (a b: Type)
+           (f:   a -> b)
+           (x:   Identity a)
+  : Identity b :=
+  f x.
+
+Instance identity_Functor
+  : Functor Identity :=
+  { map := identity_map
+  }.
+
+Definition identity_apply
+           (a b: Type)
+           (f:   Identity (a -> b))
+           (x:   Identity a)
+  : Identity b :=
+  f x.
+
+Instance identity_Apply
+  : Apply Identity :=
+  { apply := identity_apply
+  }.
+
+Definition identity_pure
+           (a: Type)
+           (x: a)
+  : Identity a :=
+  x.
+
+Instance identity_Applicative
+  : Applicative Identity :=
+  { pure := identity_pure
+  }.
+
+Definition identity_bind
+           (a b: Type)
+           (x:   Identity a)
+           (f:   a -> Identity b)
+  : Identity b :=
+  f x.
+
+Instance identity_Bind
+  : Bind Identity :=
+  { bind := identity_bind
+  }.
+
+Instance identity_Monad
+  : Monad Identity :=
+  {
+  }.
