theories/Control/State.v
@@ -1,0 +1,148 @@
+Require Import Coq.Logic.FunctionalExtensionality.
+Require Import Coq.Program.Basics.
+
+Require Import FreeSpec.Control.
+Require Import FreeSpec.Control.Identity.
+Require Import FreeSpec.WEq.
+
+Local Close Scope nat_scope.
+Local Open Scope free_control_scope.
+
+Definition StateT
+           (s: Type)
+           (m: Type -> Type)
+          `{Monad m}
+           (a: Type)
+  := s -> m (a * s).
+
+Definition State
+           (s: Type) :=
+  StateT s Identity.
+
+Definition state_map
+           {m: Type -> Type}
+          `{Monad m}
+           {s:   Type}
+           (a b: Type)
+           (f:   a -> b)
+           (fs:  StateT s m a)
+  : StateT s m b :=
+  fun s
+  => o <- fs s                                                      ;
+     pure (f (fst o), (snd o)).
+
+Instance state_Functor
+         (m: Type -> Type)
+        `{Monad m}
+         (s: Type)
+  : Functor (StateT s m) :=
+  { map := state_map
+  }.
+
+Definition state_apply
+           {m: Type -> Type}
+          `{Monad m}
+           {s:   Type}
+           (a b: Type)
+           (f:   StateT s m (a -> b))
+           (fs:  StateT s m a)
+  : StateT s m b :=
+  fun s
+  => u <- f s                                                       ;
+     v <- fs (snd u)                                                ;
+     pure ((fst u) (fst v), snd v).
+
+Instance state_Apply
+         (m: Type -> Type)
+        `{Monad m}
+         (s: Type)
+  : Apply (StateT s m) :=
+  { apply := state_apply
+  }.
+
+Definition state_bind
+           {m: Type -> Type}
+          `{Monad m}
+           {s:   Type}
+           (a b: Type)
+           (fs:  StateT s m a)
+           (f:   a -> StateT s m b)
+  : StateT s m b :=
+  fun x
+  => u <- fs x                                                       ;
+     pure (f (fst u)) (snd u).
+
+Instance state_Bind
+         (m: Type -> Type)
+        `{Monad m}
+         (s: Type)
+  : Bind (StateT s m) :=
+  { bind := state_bind
+  }.
+
+Definition state_pure
+           {m: Type -> Type}
+          `{Monad m}
+           {s: Type}
+           (a: Type)
+           (x: a)
+  : StateT s m a :=
+  fun t => pure (x, t).
+
+Instance state_Applicative
+         (m: Type -> Type)
+        `{Monad m}
+         (s: Type)
+  : Applicative (StateT s m) :=
+  { pure := state_pure
+  }.
+
+Instance state_Monad
+         (m: Type -> Type)
+        `{Monad m}
+         (s: Type)
+  : Monad (StateT s m) :=
+  {
+  }.
+
+Definition state_lift
+           {s: Type}
+           (m: Type -> Type)
+          `{Monad m}
+           (a: Type)
+           (x: m a)
+  : StateT s m a :=
+  fun s
+  => o <- x                                                          ;
+     pure (o, s).
+
+Instance state_MonadTrans
+         (s: Type)
+  : MonadTrans (StateT s) :=
+  { lift := state_lift
+  }.
+
+Definition runState
+           {m: Type -> Type}
+          `{Monad m}
+           {s a: Type}
+           (ps:  StateT s m a)
+           (x:   s)
+  : m (a * s) :=
+  ps x.
+
+Definition evalState
+           {m: Type -> Type}
+          `{Monad m}
+           {s a: Type}
+           (ps:  StateT s m a)
+           (x:   s)
+  : m a :=
+  fst <$> runState ps x.
+
+Definition execState
+           {s a: Type}
+           (ps:  State s a)
+           (x:   s)
+  : s :=
+  snd <$> runState ps x.
